theory/StratSymTB/Stratification.v
@@ -1,0 +1,155 @@
+Require Import Init.Wf.
+Require Import List.
+
+Require Import Games.Game.Game.
+Require Import Games.Game.Player.
+Require Import Games.Game.Draw.
+Require Import Games.Game.Win.
+Require Import Games.Game.NoWorse.
+Require Import Games.Game.Strategy.
+
+Inductive star {X} (R : X -> X -> Prop) : X -> X -> Prop :=
+  | star_nil : forall x, star R x x
+  | star_snoc : forall x y z, star R x y -> R y z -> star R x z.
+
+Record FinBranchWFOrd : Type := {
+  carrier :> Type;
+  eq_dec : forall i i' : carrier, { i = i' } + { i <> i' };
+  lt : carrier -> carrier -> Prop;
+  lt_wf : well_founded lt;
+  ancestors : carrier -> list carrier;
+  lt_ancestor : forall i j,
+    lt i j -> In i (ancestors j);
+  ancestor_lt : forall i j,
+    In i (ancestors j) -> lt i j
+  }.
+
+Record Stratification (I : FinBranchWFOrd) (G : Game) : Type := {
+  index : GameState G -> I;
+  index_decr : forall s (m : Move s),
+    { index (exec_move s m) = index s } +
+    { lt I (index (exec_move s m)) (index s) }
+  }.
+
+Require Import List.
+Import ListNotations.
+Require Import Lia.
+
+Fixpoint in_specific_map {A B} (xs : list A) :
+  (forall x, In x xs -> B) -> list B :=
+  match xs with
+  | [] => fun _ => []
+  | x :: ys => fun f =>
+    f x (or_introl eq_refl) ::
+    in_specific_map ys (fun y pf => f y (or_intror pf))
+  end.
+
+Lemma In_in_specific_map {A B} (xs : list A) (x : A)
+  (pf : In x xs) (f : forall x, In x xs -> B) :
+  In (f x pf) (in_specific_map xs f).
+Proof.
+  induction xs.
+  - destruct pf.
+  - simpl.
+    destruct pf.
+    + destruct e; left; reflexivity.
+    + right.
+      apply (IHxs i (fun x pf => f x (or_intror pf))).
+Qed.
+
+Lemma in_specific_map_In {A B} (xs : list A) (y : B)
+  (f : forall x, In x xs -> B) :
+  In y (in_specific_map xs f) ->
+  exists (x : A) (pf : In x xs),
+  f x pf = y.
+Proof.
+  induction xs; intro pf.
+  - destruct pf.
+  - simpl in pf.
+    destruct pf.
+    + exists a.
+      eexists; exact H.
+    + destruct (IHxs _ H) as [x [pf Hxpf]].
+      exists x.
+      eexists; exact Hxpf.
+Qed.
+
+Lemma in_specific_map_iff {A B} (xs : list A) (y : B)
+  (f : forall x, In x xs -> B) :
+  In y (in_specific_map xs f) <->
+  exists (x : A) (pf : In x xs),
+  f x pf = y.
+Proof.
+  split.
+  - apply in_specific_map_In.
+  - intros [x [pf Hpf]].
+    rewrite <- Hpf.
+    apply In_in_specific_map.
+Qed.
+
+Fixpoint compute_all_ancestors_aux {I : FinBranchWFOrd} (i : I)
+  (a : Acc (lt I) i) {struct a} : list I.
+Proof.
+  destruct a.
+  apply (cons i).
+  apply (nodup (eq_dec I)).
+  refine (concat _).
+  unshelve eapply in_specific_map;
+    [| exact (ancestors I i) |].
+  intros x' pf.
+  apply (compute_all_ancestors_aux I x').
+  apply H.
+  apply ancestor_lt.
+  exact pf.
+Defined.
+
+Definition compute_all_ancestors {I : FinBranchWFOrd} (i : I) : list I :=
+  compute_all_ancestors_aux i
+  (lt_wf I i).
+
+Fixpoint compute_all_ancestors_aux_star {I : FinBranchWFOrd} (i j : I) a {struct a} :
+  In j (compute_all_ancestors_aux i a) -> star (lt I) j i.
+Proof.
+  intro pf.
+  destruct a; simpl in pf.
+  destruct pf.
+  - subst. apply star_nil.
+  - rewrite nodup_In in H.
+    rewrite in_concat in H.
+    destruct H as [xs [Hxs1 Hxs2]].
+    rewrite in_specific_map_iff in Hxs1.
+    destruct Hxs1 as [i' [pf Hi'pf]].
+    rewrite <- Hi'pf in Hxs2; clear Hi'pf.
+    apply compute_all_ancestors_aux_star in Hxs2.
+    apply ancestor_lt in pf.
+    apply star_snoc with (y := i'); auto.
+Qed.
+
+Fixpoint star_compute_all_ancestors_aux {I : FinBranchWFOrd} (i j : I) a
+  (pf : star (lt I) j i) {struct pf} :
+  In j (compute_all_ancestors_aux i a).
+Proof.
+  destruct pf.
+  - destruct a; left.
+    reflexivity.
+  - destruct a; right.
+    rewrite nodup_In.
+    rewrite in_concat.
+    apply lt_ancestor in H.
+    exists (compute_all_ancestors_aux y
+      (a y (ancestor_lt I y z H))); split.
+    + rewrite in_specific_map_iff.
+      exists y, H.
+      reflexivity.
+    + apply star_compute_all_ancestors_aux; auto.
+Qed.
+
+Lemma compute_all_ancestors_correct {I : FinBranchWFOrd} (i j : I) :
+  In j (compute_all_ancestors i) <-> star (lt I) j i.
+Proof.
+  split.
+  - apply compute_all_ancestors_aux_star.
+  - apply star_compute_all_ancestors_aux.
+Qed.
+
+
